Working on Globals.

low/print.ml
@@ -1,5 +1,22 @@
 
+open Low
+
+let char_list_to_string str =
+  String.concat "" (List.map (String.make 1) str)
+
 let print_SExpRec_pointer = function
     | None -> "NULL"
     | Some i -> string_of_int i
+
+let print_result = function
+  | Result_success (s, g) ->
+    print_endline "Success"
+  | Result_error (s, str) ->
+    print_endline ("Error: " ^ char_list_to_string str)
+  | Result_impossible (s, str) ->
+    print_endline ("Impossible! Please report. " ^ char_list_to_string str)
+  | Result_not_implemented str ->
+    print_endline ("Not implemented: " ^ char_list_to_string str)
+  | Result_bottom s ->
+    print_endline "Stopped because of lack of fuel."
 
