low/runR.ml
@@ -1,19 +1,4 @@
 
-open Low
-
-let char_list_to_string str =
-  String.concat "" (List.map (String.make 1) str)
-
 let _ =
-  match setup_Rmainloop max_int empty_state with
-  | Result_success (s, g) ->
-    print_endline "Success"
-  | Result_error (s, str) ->
-    print_endline ("Error: " ^ char_list_to_string str)
-  | Result_impossible (s, str) ->
-    print_endline ("Impossible! Please report. " ^ char_list_to_string str)
-  | Result_not_implemented str ->
-    print_endline ("Not implemented: " ^ char_list_to_string str)
-  | Result_bottom s ->
-    print_endline "Stopped because of lack of fuel."
+  Print.print_result (Low.setup_Rmainloop max_int Low.empty_state)
 
