low/Globals.v
@@ -1,0 +1,289 @@
+(** Globals.
+  * Lists all global variables used in the C source code of R,
+  * that are initialised, then never changed. **)
+
+
+Require Export RinternalsAux.
+
+
+(** Global variables that are initialised once, then treated as
+  constants.  They are initialised in the file Rinit.v. **)
+Record Globals := make_Globals {
+    R_NilValue : SExpRec_pointer ;
+
+    R_EmptyEnv : SExpRec_pointer ;
+    R_BaseEnv : SExpRec_pointer ;
+    R_GlobalEnv : SExpRec_pointer ;
+    R_BaseNamespace : SExpRec_pointer ;
+    R_BaseNamespaceName : SExpRec_pointer ;
+    R_BaseSymbol : SExpRec_pointer ;
+    R_NamespaceRegistry : SExpRec_pointer ;
+    R_NamespaceSymbol : SExpRec_pointer ;
+    R_MethodsNamespace : SExpRec_pointer ;
+
+    R_TrueValue : SExpRec_pointer ;
+    R_FalseValue : SExpRec_pointer ;
+    R_LogicalNAValue : SExpRec_pointer ;
+
+    R_UnboundValue : SExpRec_pointer ;
+    R_MissingArg : SExpRec_pointer ;
+    R_DotsSymbol : SExpRec_pointer ;
+    R_QuoteSymbol : SExpRec_pointer ;
+
+    R_ClassSymbol : SExpRec_pointer ;
+    R_RowNamesSymbol : SExpRec_pointer
+  }.
+
+
+(** We are going to update structures of type [Globals] a lot of time
+ * in Module Rinit. There is unfortunately no [{o with f := v}] syntax
+ * in Coq. As we are going to need it (as it helps avoid mistakes in
+ * this particular case), we implement a specialised version in Ltac. **)
+
+(** Here follows a list of all the constructors of [Globals]. **)
+Definition Globals_constructors :=
+  [ R_NilValue ;
+    R_EmptyEnv ;
+    R_BaseEnv ;
+    R_GlobalEnv ;
+    R_BaseNamespace ;
+    R_BaseNamespaceName ;
+    R_BaseSymbol ;
+    R_NamespaceRegistry ;
+    R_NamespaceSymbol ;
+    R_MethodsNamespace ;
+    R_TrueValue ;
+    R_FalseValue ;
+    R_LogicalNAValue ;
+    R_UnboundValue ;
+    R_MissingArg ;
+    R_DotsSymbol ;
+    R_QuoteSymbol ;
+    R_ClassSymbol ;
+    R_RowNamesSymbol ].
+
+(** The following property translates the [{o with f := v}] syntax from
+ * OCaml as a property. Intuitively, we have
+ * [globals_with g [(C1, p1);... ; (Cn, pn)] g'] if and only if
+ * [g' = {g with C1 := p1, ..., Cn := pn}]. **)
+Record globals_with g (L : list ((Globals -> SExpRec_pointer) * SExpRec_pointer)) g' := {
+    globals_with_in : forall C p,
+      Mem (C, p) L ->
+      C g' = p ;
+    globals_with_out : forall C,
+      (forall p, ~ Mem (C, p) L) ->
+      Mem C Globals_constructors ->
+      C g' = C g ;
+  }.
+
+(** Solves a goal of the form [{g' | globals_with g L g'}] with an instanciated [L]. **)
+Ltac solve_globals_with :=
+  let g := fresh "g" in
+  refine (let g := make_Globals in _); repeat refine (let g := g _ in _);
+  exists g; constructors;
+  [ let M := fresh "M" in introv M;
+    repeat (inverts M as M; [ simpl; reflexivity |]); inverts M
+  | let NM := fresh "NM" in introv NM;
+    let M := fresh "M" in introv M;
+    repeat (inverts M as M; [ try solve [ simpl; reflexivity
+                                        | false NM; repeat constructors ] |]); inverts M ].
+
+(** The following tactics builds a term [g'] such that [globals_with g L g']. **)
+Ltac build_globals_with g L :=
+  let g' := fresh "g" in
+  exact (proj1_sig (ltac:(solve_globals_with) : { g' | globals_with g L g' })).
+
+Delimit Scope globals_scope with globals.
+
+(** Hidding the tactic under a readable notation. **)
+Notation "'{{!' g 'with' L '!}}'" :=
+  (ltac:(build_globals_with g L)) : globals_scope.
+
+Open Scope globals.
+
+(** A dummy element of [Globals], in which all fields are mapped to [NULL]. **)
+Definition empty_globals : Globals.
+  refine (proj1_sig (P := fun g => forall C, Mem C Globals_constructors -> C g = NULL) _).
+  refine (let g := make_Globals in _). repeat refine (let g := g _ in _). exists g.
+  introv M. repeat (inverts M as M; [simpl; reflexivity|]). inverts M.
+Defined.
+
+Lemma empty_globals_constructors : forall C,
+  Mem C Globals_constructors ->
+  C empty_globals = NULL.
+Proof.
+  introv M. repeat (inverts M as M; [ reflexivity |]). inverts M.
+Qed.
+
+(** A dummy pointer different than [NULL]. **)
+Definition dummy_not_NULL : { p : SExpRec_pointer | p <> NULL }.
+  exists (Some arbitrary : SExpRec_pointer). discriminate.
+Defined.
+
+Lemma No_duplicates_Globals_constructors : No_duplicates Globals_constructors.
+Proof.
+  repeat constructors;
+  abstract
+    (introv M; repeat (inverts M as M; [
+       match type of M with ?C1 = ?C2 =>
+         set (g := {{! empty_globals with [(C1, proj1_sig dummy_not_NULL)] !}});
+         asserts E: (C1 g = C2 g); [ rewrite M; reflexivity | inverts E ]
+       end |]);
+     inverts M).
+Qed.
+
+(** The notation [{{! g with L !}}] is useful. Unfortunately, it is actually a
+ * tactic, and only works if the list [L] is known at extraction time. There
+ * exists a place in the module Rinit in which the list [L] is computed at
+ * execution time (its constructors are however known before, but it would make
+ * the definition less readable that way). We here propose need something else
+ * to deal with such list: having a computable equivalent of [{{! g with L !}}].
+ * Note that as [{{! g with L !}}] is faster at execution time, it is still
+ * preferable when possible. **)
+
+Definition Globals_with (g : Globals) (C : Globals -> SExpRec_pointer) (v : SExpRec_pointer) :
+    Mem C Globals_constructors ->
+    { g' | globals_with g [(C, v)] g' }.
+  introv M0. lets M: M0. lets ND: No_duplicates_Globals_constructors.
+  repeat match type of M with
+    | Mem _ [?C0] =>
+      let E := fresh "E" in
+      asserts E: (C = C0);
+      [ inverts M as M; [ reflexivity | inverts M ]
+      | clear M; rewrite E; solve_globals_with ]
+    | Mem _ ?l =>
+      let M1 := fresh "M" in
+      (forwards M1: divide_list_Mem M; [ apply surjective_pairing |]);
+      let ND1 := fresh "ND" in let ND2 := fresh "ND" in
+      (forwards (ND1&ND2): divide_list_No_duplicates ND; [ reflexivity |]);
+      let g' := fresh "g" in
+      set (g' :=
+        let L := map (fun C => (C, proj1_sig dummy_not_NULL)) (fst (divide_list l)) in
+        ltac:(solve_globals_with) : { g' | globals_with empty_globals L g' });
+      let E := fresh "E" in
+      destruct (C (proj1_sig g')) eqn: E;
+      [ (* [Some] case: we are in the first list. *)
+        asserts M': (Mem C (fst (divide_list l)));
+        [ inverts M1 as M1;
+          [ eassumption
+          | erewrite globals_with_out in E;
+            [ rewrite empty_globals_constructors in E; [ inverts E | apply M0 ]
+            | apply (proj2_sig g')
+            | let MA := fresh "M" in let M2 := fresh "M" in let E' := fresh "E" in
+              introv MA; forwards (?&M2&E'): Mem_map_inv (rm MA); inverts E';
+              applys divide_list_Mem_No_duplicates M ND M2 M1; reflexivity
+            | apply M0 ]
+        ]
+        | clear ND ND2 M; rename M' into M; rename ND1 into ND ]
+      | (* [None] case: we are in the second list. *)
+        asserts M': (Mem C (snd (divide_list l))) ;
+        [ inverts M1 as M1;
+          [ erewrite globals_with_in with (p := proj1_sig dummy_not_NULL) in E;
+            [ inverts E
+            | apply (proj2_sig g')
+            | apply Mem_map with (f := fun C => (C, proj1_sig dummy_not_NULL)); apply M1 ]
+          | eassumption ]
+        | clear ND ND1 M; rename M' into M; rename ND2 into ND ]
+      ];
+      clear M1 E g'; simpl in M
+  end.
+Defined.
+
+Lemma Globals_constructors_all : forall g g',
+  (forall C, Mem C Globals_constructors -> C g = C g') ->
+  g = g'.
+Proof.
+  introv F. destruct g, g'.
+  let rec t l :=
+    match l with
+    | nil => reflexivity
+    | ?C :: ?l' =>
+      forwards E: F C;
+      [ repeat constructors
+      | simpl in E; rewrite E; clear E ];
+      t l'
+    end in
+  let l := eval unfold Globals_constructors in Globals_constructors in
+  t l.
+Qed.
+
+Lemma globals_with_empty : forall g g',
+  globals_with g nil g' <-> g = g'.
+Proof.
+  iff G.
+  - apply Globals_constructors_all. introv M.
+    symmetry. applys~ globals_with_out G. introv M'. inverts M'.
+  - constructors.
+    + introv M. inverts M.
+    + introv F M. rewrite~ G.
+Qed.
+
+Lemma globals_with_transitive : forall g1 g2 g3 L1 L2 L1',
+  globals_with g1 L1 g2 ->
+  (forall C v, Mem (C, v) L1 -> Mem C Globals_constructors) ->
+  globals_with g2 L2 g3 ->
+  Filter (fun C_v => ~ exists v, Mem (fst C_v, v) L2) L1 = L1' ->
+  globals_with g1 (L1' ++ L2) g3.
+Proof.
+  introv G1 I G2 F. rewrite <- F. clear F. constructors.
+  - introv M. rewrite Mem_app_or_eq in M. inverts M as M.
+    + forwards (M'&NE): Filter_Mem_inv M.
+      erewrite globals_with_out with (g := g2).
+      * erewrite globals_with_in.
+        -- reflexivity.
+        -- apply G1.
+        -- autos~.
+      * apply G2.
+      * rew_logic~ in NE.
+      * applys I M'.
+    + erewrite globals_with_in.
+      * reflexivity.
+      * apply G2.
+      * autos~.
+  - introv NM M. erewrite globals_with_out with (g := g2).
+    + erewrite globals_with_out with (g := g1).
+      * reflexivity.
+      * apply~ G1.
+      * introv M1. eapply NM. rewrite Mem_app_or_eq. left. applys Filter_Mem M1.
+        introv (v&M2). false NM. rewrite Mem_app_or_eq. right*.
+      * autos~.
+    + apply G2.
+    + introv M'. false NM. rewrite Mem_app_or_eq. right*.
+    + autos~.
+Qed.
+
+Lemma globals_with_transitive_step : forall g1 g2 g3 C1 v1 L2,
+  globals_with g1 [(C1, v1)] g2 ->
+  Mem C1 Globals_constructors ->
+  (forall v, ~ Mem (C1, v) L2) ->
+  globals_with g2 L2 g3 ->
+  globals_with g1 ((C1, v1) :: L2) g3.
+Proof.
+  introv G1 M F G2. forwards~ G: globals_with_transitive G1 G2.
+  - introv M'. inverts M' as M'.
+    + autos~.
+    + inverts M'.
+  - rewrite Filter_cons in G. rewrite Filter_nil in G. cases_if as I.
+    + apply G.
+    + lets (v&MI): (rm I). false* F.
+Qed.
+
+Definition Globals_with_list (g : Globals) (L : list ((Globals -> SExpRec_pointer) * SExpRec_pointer)) :
+    (forall C v, Mem (C, v) L -> Mem C Globals_constructors) ->
+    No_duplicates (map fst L) ->
+    { g' | globals_with g L g' }.
+  introv F ND. gen g. induction L; introv.
+  - exists g. rewrite~ globals_with_empty.
+  - destruct a as [C v]. asserts M: (Mem C Globals_constructors).
+    + apply~ F.
+    + forwards IHg: IHL (proj1_sig (Globals_with g C v M)).
+      * introv M'. apply~ F. apply* Mem_next.
+      * inverts~ ND.
+      * exists (proj1_sig (Globals_with (proj1_sig IHg) C v M)).
+        apply~ globals_with_transitive_step.
+        -- refine (proj2_sig (Globals_with _ _ _ _)). apply~ F.
+        -- introv M'. rew_list in ND. inverts ND as NM ND. false NM.
+           applys Mem_map M'.
+        -- refine (proj2_sig (Globals_with _ _ _ _)).
+Defined.
+
